
\documentclass{article}
\usepackage{amsmath, amssymb}
\usepackage{physics}
\usepackage{geometry}
\geometry{margin=1in}

\begin{document}

\section*{Vector Calculus and Differential Equations Problems}

\subsection*{Problem 1: Coplanarity of Three Vectors}

The three vectors \( \vec{a}, \vec{b}, \vec{c} \) are coplanar if and only if their scalar triple product is zero:
\[
\vec{a} \cdot (\vec{b} \times \vec{c}) = 0
\]

\noindent\textbf{Final Answer: } \fbox{$\vec{a} \cdot (\vec{b} \times \vec{c}) = 0$}

\bigskip

\subsection*{Problem 2: Tangent Plane to a Surface}

Given the surface:
\[
z = 2e^{-x} \sin(2y)
\]
At point \( \left(0, \frac{\pi}{12}, 1\right) \):

\[
f_x = -2e^{-x} \sin(2y), \quad f_y = 4e^{-x} \cos(2y)
\]
\[
f_x(0, \pi/12) = -1, \quad f_y(0, \pi/12) = 2\sqrt{3}
\]
\[
z - 1 = -x + 2\sqrt{3}\left(y - \frac{\pi}{12} \right) \Rightarrow x - 2\sqrt{3}y + z = \frac{-\sqrt{3} \pi + 6}{6}
\]

\noindent\textbf{Final Answer: } \fbox{$x - 2\sqrt{3}y + z = \frac{-\sqrt{3} \pi + 6}{6}$}

\bigskip

\subsection*{Problem 3: Divergence of a Scalar-Vector Product}

Given \( f(x,y,z) = x^2 + y^2 + z^2 \) and \( \vec{r} = x\hat{i} + y\hat{j} + z\hat{k} \), compute:
\[
\nabla \cdot (f\vec{r}) = (\nabla f) \cdot \vec{r} + f(\nabla \cdot \vec{r}) = 2f + 3f = 5f
\]

\noindent\textbf{Final Answer: } \fbox{$5f$}

\bigskip

\subsection*{Problem 4: Curl of a Cross Product}

Given constant vector \( \vec{a} \) and \( \vec{r} = x\hat{i} + y\hat{j} + z\hat{k} \):

\[
\nabla \times (\vec{a} \times \vec{r}) = \vec{a} (\nabla \cdot \vec{r}) - (\vec{a} \cdot \nabla) \vec{r} = 3\vec{a} - \vec{a} = 2\vec{a}
\]

\noindent\textbf{Final Answer: } \fbox{$2\vec{a}$}

\bigskip

\subsection*{Problem 5: Chain Rule for Composite Function \( f(x(t), y(t)) \)}

Given:
\[
f(x, y) = x \cos y + e^x \sin y, \quad x = t^2 + 1, \quad y = t^3 + t
\]
Using the chain rule:
\[
\frac{df}{dt} = \frac{\partial f}{\partial x} \frac{dx}{dt} + \frac{\partial f}{\partial y} \frac{dy}{dt}
\]
At \( t = 0 \), we compute:
\[
\frac{dx}{dt} = 0, \quad \frac{dy}{dt} = 1, \quad \frac{\partial f}{\partial x} = 1, \quad \frac{\partial f}{\partial y} = e
\]
\[
\frac{df}{dt} = 0 + e = e
\]

\noindent\textbf{Final Answer: } \fbox{$e$}

\bigskip

\subsection*{Problem 6: First-Order Linear ODE with Initial Condition}

Given:
\[
\cos(x) + y \sin(x) = \cos(x) \frac{dy}{dx}, \quad y(\pi) = 0
\]
Rewriting:
\[
\frac{dy}{dx} - y \tan(x) = 1
\]
Integrating factor: \( \mu(x) = \cos x \), then:
\[
\frac{d}{dx}(y \cos x) = \cos x \Rightarrow y \cos x = \sin x + C
\Rightarrow y = \tan x
\Rightarrow y\left(\frac{\pi}{3}\right) = \sqrt{3}
\]

\noindent\textbf{Final Answer: } \fbox{$\sqrt{3}$}

\bigskip

\subsection*{Problem 7: Second-Order ODE with Change of Variables}

Given:
\[
x^2 y'' + 5x y' + 3y = \ln(x), \quad x = e^t
\]
Transforming:
\[
\frac{d^2y}{dt^2} + 4\frac{dy}{dt} + 3y = t, \quad \text{solution: } y = Ae^{-t} + Be^{-3t} + \frac{1}{3}t - \frac{4}{9}
\]
Back-substitute \( t = \ln x \):
\[
y(x) = \frac{A}{x} + \frac{B}{x^3} + \frac{1}{3} \ln x - \frac{4}{9}
\]

\noindent\textbf{Final Answer: } \fbox{$\frac{A}{x} + \frac{B}{x^3} + \frac{1}{3} \ln x - \frac{4}{9}$}

\bigskip

\subsection*{Problem 8: Taylor Series Expansion about a Point \( x = a \)}

The Taylor series is:
\[
f(x) = f(a) + \frac{(x - a)}{1!} f'(a) + \frac{(x - a)^2}{2!} f''(a) + \cdots + \frac{(x - a)^n}{n!} f^{(n)}(a) + \cdots
\]

\noindent\textbf{Final Answer: } \fbox{(d)}

\bigskip

\subsection*{Problem 9: Condition for Analyticity of Complex Function}

For \( f(z) = u(x, y) + iv(x, y) \), \( z = x + iy \), the Cauchy-Riemann equations must hold:
\[
\frac{\partial u}{\partial x} = \frac{\partial v}{\partial y}, \quad \frac{\partial u}{\partial y} = -\frac{\partial v}{\partial x}
\]

\noindent\textbf{Final Answer: } \fbox{(b)}

\end{document}
